Move code

theories/Dot/lr/lr_lemma.v
@@ -5,7 +5,138 @@ From iris.program_logic Require Import language.
 From D Require Import swap_later_impl.
 From D.Dot Require Import rules synLemmas unary_lr.
 
-Implicit Types (L T U: ty) (v: vl) (e: tm) (d: dm) (ds: dms) (Γ : ctx).
+Implicit Types (L T U: ty) (v: vl) (e: tm) (d: dm) (ds: dms) (Γ : ctx) (ρ : env).
+
+(** * When is a context weaker than another? *)
+(* Likely, this should be an iProp. *)
+Definition ctx_sub `{HdlangG: dlangG Σ} Γ1 Γ2 : Prop := ∀ ρ, ⟦ Γ1 ⟧* ρ -∗ ⟦ Γ2 ⟧* ρ.
+Infix "<:*" := ctx_sub (at level 70).
+
+Section CtxSub.
+  Context `{HdlangG: dlangG Σ}.
+
+  (** * Basic lemmas about [ctx_sub]. *)
+  (* TODO: Make this into a structural typing rule? *)
+
+  (** Typing is contravariant in [Γ]. *)
+  Lemma ietp_weaken_ctx {T e Γ1 Γ2} (Hweak : Γ1 <:* Γ2):
+    Γ2 ⊨ e : T -∗ Γ1 ⊨ e : T.
+  Proof. iIntros "#HT1 !>" (ρ) "#HG". iApply "HT1". by iApply Hweak. Qed.
+
+  (** The strength ordering of contexts lifts the strength ordering of types. *)
+  Lemma env_lift_sub f g {Γ} (Hweak: ∀ T ρ v, ⟦ f T ⟧ ρ v -∗ ⟦ g T ⟧ ρ v):
+    f <$> Γ <:* g <$> Γ.
+  Proof.
+    elim: Γ => [//| T Γ IH] ρ. cbn; rewrite (Hweak T).
+    iIntros "[HG $]". by iApply IH.
+  Qed.
+
+  Lemma env_lift_sub' f g Γ {Γ1 Γ2}:
+    Γ1 = f <$> Γ → Γ2 = g <$> Γ →
+    (∀ T ρ v, ⟦ f T ⟧ ρ v -∗ ⟦ g T ⟧ ρ v) →
+    Γ1 <:* Γ2.
+  Proof. move => -> -> Hweak. exact: env_lift_sub. Qed.
+
+  (** A left inverse of TLater. Sometimes written ⊲. *)
+  Definition unTLater T : ty := match T with TLater T' => T' | _ => T end.
+
+  Definition unTLater_TLater T: unTLater (TLater T) = T := reflexivity _.
+  Global Instance: Cancel (=) unTLater TLater. Proof. exact: unTLater_TLater. Qed.
+
+  (** Ordering of logical strength:
+      unTLater T <: T <: TLater (unTLater T) <: TLater T. *)
+
+  Lemma unTLater_sub T ρ v : ⟦ unTLater T ⟧ ρ v -∗ ⟦ T ⟧ ρ v.
+  Proof. case: T => //= T. by auto. Qed.
+
+  Lemma TLater_unTLater_sub T ρ v : ⟦ T ⟧ ρ v -∗ ⟦ TLater (unTLater T) ⟧ ρ v.
+  Proof. destruct T; iIntros "$". Qed.
+
+  Lemma TLater_unTLater_sub_TLater T ρ v :
+    ⟦ TLater (unTLater T) ⟧ ρ v -∗ ⟦ TLater T ⟧ ρ v.
+  Proof. destruct T; iIntros "$". Qed.
+
+  (** Lift the above ordering to environments. *)
+  Lemma TLater_ctx_sub Γ : Γ <:* TLater <$> Γ.
+  Proof. apply (env_lift_sub' id TLater Γ); rewrite ?list_fmap_id; auto. Qed.
+
+  Lemma TLater_unTLater_ctx_sub Γ : Γ <:* TLater <$> (unTLater <$> Γ).
+  Proof.
+    rewrite -list_fmap_compose.
+    apply (env_lift_sub' id (TLater ∘ unTLater) Γ), TLater_unTLater_sub;
+      by rewrite ?list_fmap_id.
+  Qed.
+
+  Lemma TLater_unTLater_TLater_ctx_sub Γ :
+    TLater <$> (unTLater <$> Γ) <:* TLater <$> Γ.
+  Proof.
+    rewrite -list_fmap_compose.
+    apply env_lift_sub, TLater_unTLater_sub_TLater.
+  Qed.
+
+  Lemma ctx_sub_unTLater Γ : unTLater <$> Γ <:* Γ.
+  Proof.
+    apply (env_lift_sub' unTLater id Γ), unTLater_sub;
+      by rewrite ?list_fmap_id.
+  Qed.
+
+  Lemma env_TLater_commute Γ ρ : ⟦ TLater <$> Γ ⟧* ρ ⊣⊢ ▷ ⟦ Γ ⟧* ρ.
+  Proof.
+    elim: Γ ρ => [| T Γ IH] ρ; cbn; [|rewrite IH later_and];
+      iSplit; by [iIntros "$" | iIntros "_"].
+  Qed.
+End CtxSub.
+
+Section LambdaIntros.
+  Context `{HdlangG: dlangG Σ}.
+
+  Lemma T_Forall_I_Strong {Γ} T1 T2 e:
+    T1.|[ren (+1)] :: (unTLater <$> Γ) ⊨ e : T2 -∗
+    (*─────────────────────────*)
+    Γ ⊨ tv (vabs e) : TAll T1 T2.
+  Proof.
+    iIntros "#HeT !>" (ρ) "#HG /=".
+    rewrite -wp_value'. iExists _; iSplit; first done.
+    iIntros "!>" (v); rewrite -(decomp_s _ (v .: ρ)).
+    (* Factor ⪭ out of [⟦ Γ ⟧* ρ] before [iNext]. *)
+    rewrite TLater_unTLater_ctx_sub env_TLater_commute. iNext.
+    iIntros "#Hv".
+    iApply ("HeT" $! (v .: ρ) with "[$HG]").
+    by rewrite (interp_weaken_one T1 _ v) stail_eq.
+  Qed.
+
+  Lemma T_Forall_I {Γ} T1 T2 e:
+    T1.|[ren (+1)] :: Γ ⊨ e : T2 -∗
+    (*─────────────────────────*)
+    Γ ⊨ tv (vabs e) : TAll T1 T2.
+  Proof.
+    iIntros "HeT"; iApply T_Forall_I_Strong;
+      iApply (ietp_weaken_ctx with "HeT") => ρ.
+    by rewrite /= ctx_sub_unTLater.
+  Qed.
+
+  (** Lemmas about definition typing. *)
+  Lemma TVMem_I {Γ} V T v l:
+    TLater V :: Γ ⊨ tv v : T -∗
+    Γ |L V ⊨ { l := dvl v } : TVMem l T.
+  Proof.
+    iIntros "/= #Hv !>" (ρ) "[#Hg #Hw]".
+    rewrite def_interp_tvmem_eq.
+    iApply wp_value_inv'; iApply "Hv"; by iSplit.
+  Qed.
+
+  Lemma TVMem_All_I {Γ} V T1 T2 e l:
+    T1.|[ren (+1)] :: V :: Γ ⊨ e : T2 -∗
+    Γ |L V ⊨ { l := dvl (vabs e) } : TVMem l (TAll T1 T2).
+  Proof.
+    iIntros "HeT"; iApply TVMem_I.
+    (* Compared to [T_Forall_I], we must strip the later from [TLater V]. *)
+    iApply T_Forall_I_Strong;
+      iApply (ietp_weaken_ctx with "HeT") => ρ.
+    by rewrite /= ctx_sub_unTLater.
+  Qed.
+End LambdaIntros.
+
 Section Sec.
   Context `{HdlangG: dlangG Σ} Γ.
 
@@ -132,18 +263,6 @@ Section Sec.
     - iApply "HvFun". rewrite -wp_value_inv'. by iApply "Hv2Arg".
     - iIntros (v) "{HG HvFun Hv2Arg} H".
       rewrite (interp_subst_one T2 v2 v) //.
-  Qed.
-
-  Lemma T_Forall_I T1 T2 e:
-    T1.|[ren (+1)] :: Γ ⊨ e : T2 -∗
-    (*─────────────────────────*)
-    Γ ⊨ tv (vabs e) : TAll T1 T2.
-  Proof.
-    iIntros "/= #HeT !>" (vs) "#HG".
-    rewrite -wp_value'. iExists _; iSplit; first done.
-    iIntros "!> !>" (v) "#Hv"; rewrite -(decomp_s e (v .: vs)).
-    iApply ("HeT" $! (v .: vs) with "[$HG]").
-    by rewrite (interp_weaken_one T1 _ v).
   Qed.
 
   Lemma T_Mem_E e T l:
